comments are addressing, partially completed, in progress

share/pulse/examples/dice/dpe/SPDM.fst
@@ -40,7 +40,7 @@ hash (hash_algo: u32)
          (ts_digest: V.vec u8{V.length ts_digest == hash_size})
          (msg_size: u32{u32_v msg_size > 0})
          (msg: V.vec u8{V.length msg == u32_v msg_size})
-         (#ts_seq: (G.erased (Seq.seq u8)){Seq.length ts_seq == hash_size})
+         (#ts_seq: (G.erased (Seq.seq u8))(*{Seq.length ts_seq == hash_size}*))
          (#msg_seq: (G.erased (Seq.seq u8)))
          (#p_msg:perm)
         
@@ -135,7 +135,7 @@ let session_state_tag_related (s:state) (gs:g_state) : GTot bool =
   match s, gs with
    | Initialized st, G_Initialized repr
    
-   | Recv_no_sign_resp st _ _, G_Recv_no_sign_resp repr _ _ ->
+   | Recv_no_sign_resp st, G_Recv_no_sign_resp repr _ _ ->
     true
    
    | _ -> false
@@ -182,20 +182,210 @@ let valid_transition_lemma
   (tr0:trace{has_full_state_info (current_state tr0)})
   (rep:repr)
   (rep_new:repr)
+  (#b_req: G.erased (Seq.seq u8))
+  (#b_resp: G.erased (Seq.seq u8))
   : Lemma
     (requires  (G_Initialized? (current_state tr0) \/ G_Recv_no_sign_resp? (current_state tr0)) /\
                (G_Initialized? (current_state tr0) ==>
-                          (all_zeros_hash_transcript rep.transcript) /\
                           (G_Initialized rep == current_state tr0) /\
                           (rep.signing_pub_key_repr == rep_new.signing_pub_key_repr /\
-                           rep.key_size_repr = rep_new.key_size_repr )) /\
+                           rep.key_size_repr = rep_new.key_size_repr  /\
+                          hash_of hash_algo rep.transcript b_req b_resp rep_new.transcript)) /\
                 
                (G_Recv_no_sign_resp? (current_state tr0) ==>
-                          ~(all_zeros_hash_transcript rep.transcript) /\
-                          (G_Recv_no_sign_resp rep == current_state tr0) /\
+                          (exists req resp. G_Recv_no_sign_resp rep req resp == current_state tr0) /\
                           (rep.signing_pub_key_repr == rep_new.signing_pub_key_repr /\
                            rep.key_size_repr = rep_new.key_size_repr /\
-                          (exists req_size req resp_size resp hash_algo. 
-                             hash_of hash_algo rep.transcript req_size req resp_size resp rep_new.transcript)))
+                           hash_of hash_algo rep.transcript b_req b_resp rep_new.transcript))
     )
-    (ensures valid_transition tr0 (G_Recv_no_sign_resp rep_new)) = ()
+    (ensures valid_transition tr0 (G_Recv_no_sign_resp rep_new b_req b_resp)) = ()
+
+let valid_transition_lemma1
+  (tr0:trace{has_full_state_info (current_state tr0)})
+  (rep:repr)
+  (rep_new:repr)
+  (#b_req: G.erased (Seq.seq u8))
+  (#b_resp: G.erased (Seq.seq u8))
+  : Lemma
+    (requires  (G_Initialized? (current_state tr0) \/ G_Recv_no_sign_resp? (current_state tr0)) /\
+               (G_Initialized? (current_state tr0) ==>
+                          (G_Initialized rep == current_state tr0) /\
+                          (rep.signing_pub_key_repr == rep_new.signing_pub_key_repr /\
+                           rep.key_size_repr = rep_new.key_size_repr /\
+                           hash_of hash_algo rep.transcript b_req b_resp rep_new.transcript)) /\
+                
+               (G_Recv_no_sign_resp? (current_state tr0) ==>
+                          (exists req resp. G_Recv_no_sign_resp rep req resp == current_state tr0) /\
+                          (rep.signing_pub_key_repr == rep_new.signing_pub_key_repr /\
+                           rep.key_size_repr = rep_new.key_size_repr /\
+                           hash_of hash_algo rep.transcript b_req b_resp rep_new.transcript))
+    )
+    (ensures valid_transition tr0 (G_Recv_sign_resp rep_new b_req b_resp)) = ()
+
+fn
+no_sign_resp_aux
+  (ctx:parser_context{u32_v ctx.resp_size > 0})
+  (req_size: u32{u32_v req_size > 0})
+  (req:V.vec u8 { V.length req == u32_v req_size })
+  (c:state)
+  (st:st)
+  (rep:repr)
+  (res:spdm_measurement_result_t)
+  (#tr0:trace{has_full_state_info (current_state tr0)})
+  (#b_req: G.erased (Seq.seq u8))
+  (#b_resp: G.erased (Seq.seq u8))
+  (#p_req : perm)
+  (#p_resp:perm)
+  requires parser_post1 ctx res false **
+           V.pts_to req #p_req b_req **
+           V.pts_to ctx.resp #p_resp b_resp **
+           V.pts_to st.session_transcript rep.transcript **
+           V.pts_to st.signing_pub_key rep.signing_pub_key_repr **
+           pure (st.key_size == rep.key_size_repr /\
+                (c == Initialized st \/ c == Recv_no_sign_resp st) /\
+                (rep.transcript == (current_transcript tr0)) /\
+                (rep.signing_pub_key_repr == (current_key tr0)) /\
+                (rep.key_size_repr == (current_key_size tr0)) /\
+                (G_Recv_no_sign_resp? (current_state tr0) \/ G_Initialized? (current_state tr0)) /\
+                (G_Initialized? (current_state tr0) ==>
+                          (G_Initialized rep == current_state tr0)) /\
+                (G_Recv_no_sign_resp? (current_state tr0) ==>
+                          (exists b_req' b_resp'. G_Recv_no_sign_resp rep b_req' b_resp' == current_state tr0)) /\
+                res.status == Success) **
+           C.ghost_pcm_pts_to 
+                  (get_state_data c).g_trace_ref
+                  (Some #perm 1.0R, tr0)
+
+           
+  returns ret: spdm_measurement_result_t & state
+   
+   ensures  V.pts_to req #p_req b_req **
+            V.pts_to ctx.resp #p_resp b_resp **
+            parser_post1 ctx (fst ret) false **
+             (exists* tr1.
+                  spdm_inv (snd ret) (get_state_data (snd ret)).g_trace_ref tr1 **
+                  pure ((fst ret).status == Success ==>
+                                      state_change_success_no_sign tr0 tr1 /\
+                                      hash_result_success_no_sign tr0 tr1 #b_req #b_resp))
+{
+  let curr_state_data = get_state_data c;
+    let curr_state_transcript:V.vec u8 = curr_state_data.session_transcript;
+    let curr_state_signing_pub_key = curr_state_data.signing_pub_key;
+    let curr_state_key_size = curr_state_data.key_size;
+      //get the ghost transcript
+    let curr_g_transcript = current_transcript tr0;
+      
+    let curr_g_key = current_key tr0;
+    let curr_g_key_size = current_key_size tr0;
+    
+    rewrite (V.pts_to st.session_transcript rep.transcript) as
+                  (V.pts_to curr_state_transcript rep.transcript);
+        
+    rewrite (V.pts_to curr_state_transcript rep.transcript) as
+                (V.pts_to curr_state_transcript curr_g_transcript);
+    
+    assert_ (pure(Seq.length curr_g_transcript == hash_size));
+    let new_g_transcript' = hash_spec hash_algo curr_g_transcript b_req;
+    let new_g_transcript = hash_spec hash_algo new_g_transcript' b_resp;
+
+    assert_ (pure(V.length curr_state_transcript == hash_size /\
+                  u32_v req_size > 0 /\
+                  V.length req == u32_v req_size)); 
+    
+    assert_ (V.pts_to curr_state_transcript curr_g_transcript);
+    assert_ (V.pts_to req #p_req b_req);
+
+    hash hash_algo curr_state_transcript req_size req #curr_g_transcript #b_req #p_req;
+
+    assert_ (pure(V.length curr_state_transcript == hash_size /\
+                  u32_v ctx.resp_size > 0 /\
+                  V.length ctx.resp == u32_v ctx.resp_size)); 
+
+    hash hash_algo curr_state_transcript ctx.resp_size ctx.resp #new_g_transcript' #b_resp #p_resp;
+
+    let rep_new = {key_size_repr = curr_g_key_size; signing_pub_key_repr = curr_g_key; transcript = new_g_transcript};
+
+    //Trace ref creation-----------------------------------------------------------------------------------------------------------
+    //new trace----------------------------------------------------------------------------------------------------------------
+    //bring in a lemma to prove this
+    valid_transition_lemma tr0 rep rep_new;
+    assert_ (pure(valid_transition tr0 (G_Recv_no_sign_resp rep_new b_req b_resp)));
+
+    let tr1 = next_trace tr0 (G_Recv_no_sign_resp rep_new b_req b_resp);
+
+    extend_trace ((get_state_data c).g_trace_ref) tr0 ((G_Recv_no_sign_resp rep_new b_req b_resp));
+
+     //New state data record creation
+    //----------------------------------------------------------------------------------------------------------------------------
+    let new_st = {key_size = curr_state_key_size; 
+                    signing_pub_key = curr_state_signing_pub_key; 
+                    session_transcript = curr_state_transcript;
+                    g_trace_ref = curr_state_data.g_trace_ref};
+
+
+    //Do the state change---------------------------------------------------------------------------------------------------------
+    let new_state = (Recv_no_sign_resp new_st);
+
+    with _v. rewrite (V.pts_to curr_state_transcript _v) as
+                         (V.pts_to curr_state_transcript new_g_transcript);
+
+    rewrite (V.pts_to curr_state_transcript new_g_transcript) as
+                (V.pts_to new_st.session_transcript rep_new.transcript);
+    
+     rewrite (V.pts_to st.signing_pub_key rep.signing_pub_key_repr) as
+                (V.pts_to curr_state_signing_pub_key rep.signing_pub_key_repr);
+        
+     rewrite (V.pts_to curr_state_signing_pub_key rep.signing_pub_key_repr) as
+                (V.pts_to curr_state_signing_pub_key curr_g_key);
+
+     rewrite (V.pts_to curr_state_signing_pub_key curr_g_key) as
+                (V.pts_to new_st.signing_pub_key rep_new.signing_pub_key_repr);
+
+     assert_ ( V.pts_to new_st.signing_pub_key rep_new.signing_pub_key_repr **
+                  V.pts_to new_st.session_transcript rep_new.transcript **
+                  pure (new_st.key_size == rep_new.key_size_repr));
+    
+    fold (session_state_related (Recv_no_sign_resp new_st) (G_Recv_no_sign_resp rep_new b_req b_resp));
+
+    with _v. rewrite (C.ghost_pcm_pts_to #trace_pcm_t #trace_pcm _v (pcm_elt 1.0R tr1)) as
+                         (C.ghost_pcm_pts_to (get_state_data (Recv_no_sign_resp new_st)).g_trace_ref (pcm_elt 1.0R tr1));
+    
+
+   fold (spdm_inv (Recv_no_sign_resp new_st) (get_state_data (Recv_no_sign_resp new_st)).g_trace_ref tr1);
+
+   let fin = (res, new_state);
+   fin
+}
+
+
+fn no_sign_resp1
+  (ctx:parser_context)
+  (req_size: u32{u32_v req_size > 0})
+  (req:V.vec u8 { V.length req == u32_v req_size })
+  (c:state)
+  (#tr0:trace{has_full_state_info (current_state tr0)})
+  (#b_resp: G.erased (Seq.seq u8)(*{u32_v ctx.resp_size > 0 /\ Seq.length b_resp == u32_v ctx.resp_size}*))
+  (#b_req: G.erased (Seq.seq u8)(*{Seq.length b_req == u32_v req_size}*))
+  (#p_req : perm)
+  (#p_resp:perm)
+   requires (V.pts_to req #p_req b_req **
+             V.pts_to ctx.resp #p_resp b_resp) **
+             spdm_inv c ((get_state_data c).g_trace_ref) tr0 **
+             pure (G_Recv_no_sign_resp? (current_state tr0) \/ G_Initialized? (current_state tr0))
+    returns res: (spdm_measurement_result_t & state)
+    
+    ensures V.pts_to req #p_req b_req **
+            V.pts_to ctx.resp #p_resp b_resp **
+
+            //parser related post-conditions
+            parser_post1 ctx (fst res) false  **
+           
+            //state change related post-condition 
+            (exists* tr1.
+                  spdm_inv (snd res) (get_state_data (snd res)).g_trace_ref tr1 **
+                  pure ((fst res).status == Success ==>
+                                      state_change_success_no_sign tr0 tr1 /\
+                                      hash_result_success_no_sign tr0 tr1 #b_resp #b_req ))  
+{
+  admit()
+}
